proof/TPOSR/CtxConversion.v
@@ -5,7 +5,7 @@ Require Import Lambda.TPOSR.LiftSubst.
 Require Import Lambda.TPOSR.Env.
 Require Import Lambda.TPOSR.Types.
 Require Import Lambda.TPOSR.Basic.
-Require Import Lambda.TPOSR.CtxReduction.
+Require Import Lambda.TPOSR.CtxCoercion.
 Require Import Lambda.TPOSR.RightReflexivity.
 Set Implicit Arguments.
 
@@ -13,34 +13,6 @@ Implicit Types i k m n p : nat.
 Implicit Type s : sort.
 Implicit Types A B M N T t u v : lterm.
 Implicit Types e f g : lenv.
-
-Inductive red_in_env : lenv -> lenv -> Prop :=
-  | red_env_hd : forall e t u s, e |-- t -> u : Srt_l s ->
-	red_in_env (t :: e) (u :: e)
-  | red_env_tl :
-      forall e f t, red_in_env e f -> red_in_env (t :: e) (t :: f).
-
-Hint Resolve red_env_hd red_env_tl: coc.
-
-Lemma red_env :
-  (forall e t u T, e |-- t -> u : T -> 
-  forall f, red_in_env e f -> f |-- t -> u : T).
-Proof.
-Admitted.
-
-Inductive exp_in_env : lenv -> lenv -> Prop :=
-  | exp_env_hd : forall e t u s, e |-- t -> u : Srt_l s ->
-	exp_in_env (u :: e) (t :: e)
-  | exp_env_tl :
-      forall e f t, exp_in_env e f -> exp_in_env (t :: e) (t :: f).
-
-Hint Resolve red_env_hd red_env_tl: coc.
-
-Lemma exp_env :
-  (forall e t u T, e |-- t -> u : T -> 
-  forall f, exp_in_env e f -> f |-- t -> u : T).
-Proof.
-Admitted.
 
 Inductive conv_in_env : lenv -> lenv -> Prop :=
   | conv_env_hd : forall e t u s, e |-- t ~= u : s -> 
@@ -50,28 +22,43 @@ Inductive conv_in_env : lenv -> lenv -> Prop :=
 
 Hint Resolve conv_env_hd conv_env_tl: coc.
 
+Lemma conv_in_env_coerce_in_env : forall e f, conv_in_env e f -> tposr_wf e -> coerce_in_env e f.
+Proof.
+  induction 1 ; simpl ; intros ; eauto with coc.
+  inversion H0.
+  subst.
+  pose (wf_tposr H2).
+  pose (IHconv_in_env t0).
+  apply coerce_env_tl ; auto.
+  apply wf_cons with s.
+  apply tposr_coerce_env with e ; auto.
+Qed.  
+   
+Hint Resolve conv_in_env_coerce_in_env : coc.
+
 Lemma conv_env :
   (forall e t u T, e |-- t -> u : T -> 
   forall f, conv_in_env e f -> f |-- t -> u : T).
 Proof.
-Admitted.
+  intros.
+  apply tposr_coerce_env with e ; eauto with coc ecoc.
+Qed.
 
-Corollary conv_env_eq : 
+Corollary eq_conv_env : 
   (forall e t u s, e |-- t ~= u : s -> 
   forall f, conv_in_env e f -> f |-- t ~= u : s).
 Proof.
-  induction 1 ; simpl ; intros ; auto with coc.
-
-  apply tposr_eq_tposr ; auto.
-  apply conv_env with e ; auto.
-
-  apply tposr_eq_trans with X ; auto with coc.
+  intros.
+  apply eq_coerce_env with e ; eauto with coc ecoc.
 Qed.
 
 Corollary coerce_conv_env : 
   (forall e t u s, e |-- t >-> u : s -> 
   forall f, conv_in_env e f -> f |-- t >-> u : s).
-Admitted.
+Proof.
+  intros.
+  apply coerce_coerce_env with e ; eauto with coc ecoc.
+Qed.
 
 Lemma conv_in_env_sym : forall e f, conv_in_env e f -> conv_in_env f e.
 Proof.
@@ -79,147 +66,3 @@ Proof.
 Qed.
 
 Hint Resolve conv_in_env_sym : coc.
-(*
-Inductive conv_in_env_full : lenv -> lenv -> Prop :=
-  | conv_env_full_conv : forall e f t,
-    conv_in_env_full (t :: e) (t :: f) ->
-    forall u s, e |-- t ~= u : s -> f |-- t ~= u : s -> 
-      conv_in_env_full (t :: e) (u :: f)
-  | conv_env_full_eq :
-      forall e f t, tposr_wf e -> conv_in_env_full e e
-  | conv_env_start : 
-    conv_in_env_full nil nil.
-
-Hint Resolve conv_env_full_conv conv_env_full_eq conv_env_start : coc.
-
-Lemma conv_env_full :
-  (forall e t u T, e |-- t -> u : T -> 
-  forall f, conv_in_env_full e f -> f |-- t -> u : T).
-Proof.
-  intros.
-  induction H0.
-  apply conv_env with (t0 :: f) ; auto with coc.
-  apply conv_env_hd with s ; auto.
-
-  
-
-  
-
-
-Admitted.
-*)
-(*
-Lemma ind_conv_env :
-  (forall e t T, e |-- t : T -> 
-  forall f, conv_in_env e f -> f |-- t : T) /\
-  (forall e T U s, e |-- T >> U : s -> 
-  forall f, conv_in_env e f -> f |-- T >> U : s) /\
-  (forall e U V T, e |-- U = V : T ->
-  forall f, conv_in_env e f -> f |-- U = V : T).
-Proof.
-apply typ_coerce_jeq_ind with 
-(P := fun e t T => fun H : typ e t T =>
-  forall f, conv_in_env e f -> 
-  typ f t T)
-(P0 := fun e T U s => fun H : e |-- T >> U : s =>
-  forall f, conv_in_env e f -> 
-  f |-- T >> U : s) 
-(P1 := fun e U V T => fun H : e |-- U = V : T =>
-  forall f, conv_in_env e f -> 
-  f |-- U = V : T) ;
- intros ; try (solve [destruct (H f H0) ; clear H]); 
-auto with coc core arith datatypes.
-
-inversion H ; auto with coc.
-inversion H ; auto with coc.
-
-inversion H0.
-apply type_conv with (lift 1 u) s0 ; auto with coc.
-apply type_var with s0 ; auto with coc .
-apply coerce_conv ; auto with coc.
-change (Srt s0) with (lift 1 (Srt s0)).
-apply jeq_weak with s0 ; auto.
-apply jeq_sym ; auto.
-
-apply type_var with s ; auto.
-
-inversion H1.
-apply type_weak with s0 ; auto.
-apply type_weak with s ; auto.
-
-apply type_abs with s1 s2 ; auto with coc.
-
-apply type_app with V ; auto with coc.
-
-apply type_pair with s1 s2 s3 ; auto with coc.
-
-apply type_prod with s1 ; auto with coc.
-
-apply type_sum with s1 s2 ; auto with coc.
-
-apply type_subset ; auto with coc.
-
-apply type_pi1 with V ; auto with coc.
-
-apply type_pi2 with U ; auto with coc.
-
-apply type_conv with U s ; auto with coc.
-
-inversion H1.
-apply coerce_weak with s0 ; auto with coc.
-apply coerce_weak with s' ; auto with coc.
-
-apply coerce_prod with s ; auto with coc.
-
-apply coerce_sum with s s' ; auto with coc.
-
-apply coerce_trans with B ; auto with coc.
-
-inversion H1.
-apply jeq_weak with s0 ; auto with coc.
-apply jeq_weak with s ; auto with coc.
-
-apply jeq_prod with s1 ; auto with coc.
-
-apply jeq_abs with s1 s2 ; auto with coc.
-
-apply jeq_app with A ; auto with coc.
-
-apply jeq_beta with s1 s2 ; auto with coc.
-
-apply jeq_red with A s ; auto with coc.
-
-apply jeq_exp with B s ; auto with coc.
-
-apply jeq_sum with s1 s2 ; auto with coc.
-
-apply jeq_pair with s1 s2 s3; auto with coc.
-
-apply jeq_pi1 with  B; auto with coc.
-
-apply jeq_pi1_red with s1 s2 s3; auto with coc.
-
-apply jeq_pi2 with A ; auto with coc.
-
-apply jeq_pi2_red with s1 s2 s3 ; auto with coc.
-
-apply jeq_subset ; auto with coc.
-
-apply jeq_trans with N ; auto with coc.
-
-apply jeq_conv with A s ; auto with coc.
-Qed.
-
-Lemma type_conv_env : forall e t T, e |-- t : T -> 
-  forall f, conv_in_env e f -> f |-- t : T.
-Proof (proj1 ind_conv_env).
-
-Lemma coerce_conv_env : forall e T U s, e |-- T >> U : s -> 
-  forall f, conv_in_env e f -> f |-- T >> U : s.
-Proof (proj1 (proj2 ind_conv_env)).
-
-Lemma jeq_conv_env : forall e U V T, e |-- U = V : T ->
-  forall f, conv_in_env e f -> f |-- U = V : T.
-Proof (proj2 (proj2 ind_conv_env)).
-
-*)
